RelocElfgenproof

x86/ReloctablesEncodeArchi.v
@@ -16,27 +16,17 @@ Local Open Scope bits_scope.
 
 Section WITH_IDXMAP.
 Variable  (idxmap: PTree.t Z).
+Variable (encode_reloc_info: PTree.t Z -> reloctype -> ident -> res (list byte)).
 
-Definition encode_reloc_info (t:reloctype) (symb:ident)  : res (list byte) :=
-  let te := encode_reloctype t in
-  match idxmap!symb with
-  | None => Error [MSG "Relocation target symbol doesn't exist!"; CTX symb]
-  | Some idx =>
-    if Archi.ptr64 then
-      if (0 <? idx) && (idx <? Z.pow 2 32) then
-        OK (encode_int64 (idx * (Z.pow 2 32) + te))
-      else Error (msg "Overflow in encode_reloc_info")
-    else
-      if (0 <? idx) && (idx <? Z.pow 2 24) then
-        OK (encode_int32 (idx * (Z.pow 2 8) + te))
-      else Error (msg "Overflow in encode_reloc_info")
-  end.
+Hypothesis encode_reloc_info_len: forall m r id bs,
+    encode_reloc_info m r id = OK bs ->
+    length bs = if Archi.ptr64 then 8%nat else 4%nat.
 
 Definition encode_relocentry (e:relocentry) : res (list byte) :=
   let len := if Archi.ptr64 then 64 else 32 in
   if (0 <=? e.(reloc_offset)) && (e.(reloc_offset) <? Z.pow 2 len) then
     let r_offset_bytes := if Archi.ptr64 then encode_int64 (reloc_offset e)  else  encode_int32 (reloc_offset e) in    
-    do r_info_bytes <- encode_reloc_info (reloc_type e) (reloc_symb e);
+    do r_info_bytes <- encode_reloc_info idxmap (reloc_type e) (reloc_symb e);
     if Archi.ptr64 then
       if (- (Z.pow 2 63) <=? (reloc_addend e)) && ((reloc_addend e) <? (Z.pow 2 63)) then
         OK (r_offset_bytes ++ r_info_bytes ++ encode_int64 ((reloc_addend e) mod (Z.pow 2 64)))
@@ -55,15 +45,16 @@ Lemma encode_relocentry_len: forall l e,
 Proof.
   unfold encode_relocentry.
   intros. repeat destr_in H.
-  monadInv H11. unfold encode_reloc_info in EQ.
-  repeat destr_in EQ.
+  monadInv H11. 
   unfold encode_int64. repeat rewrite app_length.
-  do 3 rewrite encode_int_length. lia.
-  monadInv H11. unfold encode_reloc_info in H11.
-  
-  repeat destr_in H11.
-  unfold encode_int32. rewrite app_length.
+  exploit encode_reloc_info_len;eauto;intros LEN.
   do 2 rewrite encode_int_length. lia.
+  monadInv H11.
+
+  monadInv H11.
+  unfold encode_int32. rewrite app_length.
+  exploit encode_reloc_info_len;eauto;intros LEN.  
+  do 1 rewrite encode_int_length. lia.
   monadInv H11.
 Qed.
 
