riscV/RelocElfgenproofArchi.v
@@ -1,11 +1,11 @@
 Require Import Coqlib Maps AST lib.Integers Values.
 Require Import Events lib.Floats Memory Smallstep.
-Require Import Asm RelocProg RelocProgramBytes RelocElf Globalenvs.
+Require Import Asm RelocProg RelocProgramBytes RelocElf RelocElfArchi Globalenvs.
 Require Import Linking RelocProgLinking RelocElfLinking Errors.
 Require Import EncDecRet RelocElfgen LocalLib RelocProgGlobalenvs.
 Require Import RelocProgSemantics RelocProgSemantics1.
 Require Import RelocProgSemantics2 RelocElfSemantics.
-Require Import SymbtableDecode ReloctablesEncode.
+Require Import SymbtableDecode ReloctablesEncode ReloctablesDecode.
 Require Import RelocProgSemanticsArchi.
 Require Import ReloctablesEncodeArchi.
 Require Import RelocElfgenproof0.
@@ -21,6 +21,44 @@ Local Open Scope string_byte_scope.
 
 
 
+Lemma decode_encode_reloctable_correct: forall n l bs m1 m2 (M: match_idxmap m1 m2),
+    (* let reloclen := if Archi.ptr64 then 24%nat else 8%nat in *)
+    length l = n ->
+    encode_reloctable m1 l = OK bs ->
+    fold_left (acc_decode_reloctable_section reloc_entry_size m2) bs (OK ([], [], 1%nat)) = OK (l, [], 1%nat).
+Proof.
+  induction n;intros.
+  rewrite length_zero_iff_nil in H. subst.
+  simpl in H0. inv H0.
+  unfold decode_reloctable_section. simpl. auto.
+
+  exploit LocalLib.length_S_inv;eauto.
+  intros (l' & a1 & A1 & B1). subst.
+  clear H.
+  unfold encode_reloctable in H0. rewrite fold_left_app in H0.
+  simpl in H0. unfold acc_reloctable in H0 at 1.
+  monadInv H0. exploit IHn;eauto.
+  intros. rewrite fold_left_app.
+
+  rewrite H. clear H EQ IHn.
+  exploit encode_relocentry_len;eauto.
+  eapply encode_reloc_info_len.  
+  intros LEN. 
+  rename x0 into l.
+  clear x.
+  eapply (ReloctablesDecodeArchi.decode_encode_relocentry encode_reloc_info decode_reloc_info) in EQ1;eauto.
+  2: eapply encode_reloc_info_len.
+  2: eapply decode_encode_reloc_info.
+
+  unfold acc_decode_reloctable_section. unfold reloc_entry_size.
+  destruct Archi.ptr64.
+  - do 25 (destruct l as [| ?b ?] ;simpl in LEN;try congruence).
+    simpl in *. rewrite EQ1. simpl. auto.
+  - do 13 (destruct l as [| ?b ?] ;simpl in LEN;try congruence).
+    simpl in *. rewrite EQ1. simpl. auto.
+Qed.
+
+
 Section WITH_INSTR_SIZE.
   Variable instr_size: instruction -> Z.
 
@@ -34,55 +72,31 @@ Let ge := RelocProgSemantics2.globalenv instr_size  prog.
 Let tge := globalenv instr_size  tprog.
 
 
-Lemma eval_addrmode_match_ge: forall ge1 ge2 a rs (MATCHGE: forall i ofs, RelocProgGlobalenvs.Genv.symbol_address ge1 i ofs = RelocProgGlobalenvs.Genv.symbol_address ge2 i ofs),
-    eval_addrmode ge1 a rs = eval_addrmode ge2 a rs.
+Lemma eval_offset_match_ge: forall ge1 ge2 ofs (MATCHGE: forall i ofs, RelocProgGlobalenvs.Genv.symbol_address ge1 i ofs = RelocProgGlobalenvs.Genv.symbol_address ge2 i ofs) ,
+    eval_offset ge1 ofs = eval_offset ge2 ofs.
 Proof.
-  unfold eval_addrmode. destruct Archi.ptr64;intros.
-  - unfold eval_addrmode64.
-    destruct a. f_equal.
-    f_equal. destr.
-    destruct p. eauto.
-  - unfold eval_addrmode32.
-    destruct a. f_equal.
-    f_equal. destr.
-    destruct p. eauto.
-Qed.
+  unfold eval_offset. intros.
+  destr.
+  eapply low_half_match_ge. eauto.
+Qed.  
 
-Lemma exec_load_match_ge: forall sz ge1 ge2 chunk m a rs rd (MATCHGE: forall i ofs, RelocProgGlobalenvs.Genv.symbol_address ge1 i ofs = RelocProgGlobalenvs.Genv.symbol_address ge2 i ofs) ,
-          exec_load sz ge1 chunk m a rs rd = exec_load sz ge2 chunk m a rs rd.
+    
+Lemma exec_load_match_ge: forall sz ge1 ge2 chunk m rs ra rd ofs (MATCHGE: forall i ofs, RelocProgGlobalenvs.Genv.symbol_address ge1 i ofs = RelocProgGlobalenvs.Genv.symbol_address ge2 i ofs) ,
+          exec_load sz ge1 chunk rs m rd ra ofs = exec_load sz ge2 chunk rs m rd ra ofs.
 Proof.
   unfold exec_load.
-  intros. erewrite eval_addrmode_match_ge.
-  eauto. auto.
+  intros.
+  erewrite eval_offset_match_ge;eauto.
 Qed.
 
-Lemma exec_store_match_ge: forall sz ge1 ge2 chunk m a rs rd l (MATCHGE: forall i ofs, RelocProgGlobalenvs.Genv.symbol_address ge1 i ofs = RelocProgGlobalenvs.Genv.symbol_address ge2 i ofs) ,
-          exec_store sz ge1 chunk m a rs rd l = exec_store sz ge2 chunk m a rs rd l.
+Lemma exec_store_match_ge: forall sz ge1 ge2 chunk m rs ra s ofs (MATCHGE: forall i ofs, RelocProgGlobalenvs.Genv.symbol_address ge1 i ofs = RelocProgGlobalenvs.Genv.symbol_address ge2 i ofs) ,
+          exec_store sz ge1 chunk rs m s ra ofs = exec_store sz ge2 chunk rs m s ra ofs.
 Proof.
   unfold exec_store.
-  intros. erewrite eval_addrmode_match_ge.
-  eauto. auto.
+  intros.
+  erewrite eval_offset_match_ge;eauto.
 Qed.
 
-Lemma eval_builtin_arg_match_ge: forall rs sp m arg varg ge1 ge2 (MATCHGE: forall i ofs, RelocProgGlobalenvs.Genv.symbol_address ge1 i ofs = RelocProgGlobalenvs.Genv.symbol_address ge2 i ofs),
-        eval_builtin_arg preg ge1 rs sp m arg varg ->
-        eval_builtin_arg preg ge2 rs sp m arg varg.
-Proof.
-  induction 2;try constructor;auto.
-  rewrite MATCHGE in H. auto.
-  rewrite MATCHGE. constructor.
-Qed.
-
-Lemma eval_builtin_args_match_ge: forall rs sp m args vargs ge1 ge2 (MATCHGE: forall i ofs, RelocProgGlobalenvs.Genv.symbol_address ge1 i ofs = RelocProgGlobalenvs.Genv.symbol_address ge2 i ofs),
-        eval_builtin_args preg ge1 rs sp m args vargs ->
-        eval_builtin_args preg ge2 rs sp m args vargs.
-Proof.
-  induction 2.
-  - constructor.
-  - econstructor.
-    eapply eval_builtin_arg_match_ge;eauto.
-    eauto.
-Qed.
 
 Lemma step_simulation: forall st1 st2 t,
     step instr_size ge st1 t st2 ->
@@ -91,11 +105,12 @@ Proof.
   intros.
   unfold ge,tge in *.
   exploit gen_reloc_elf_correct;eauto.
+  eapply decode_encode_reloctable_correct.
   unfold globalenv.
   intros (p' & D1 & E1).
   rewrite D1.
   unfold RelocProgSemantics2.globalenv in *.
-  destr_in H.
+ destr_in H.
   exploit decode_prog_code_section_correct;eauto.
   intros (p2' & D2 & E2). rewrite D2.
 
@@ -123,35 +138,12 @@ Proof.
       erewrite program_equiv_instr_map.
       eauto. eapply program_equiv_sym. eauto.
     + apply program_equiv_sym in E2.
-      destruct i;simpl in *;auto.
-      1-27: try (erewrite program_equiv_symbol_address1;eauto).
-      1-24: try (erewrite exec_load_match_ge;eauto;eapply program_equiv_symbol_address1;eauto).
-      1-12: try (erewrite exec_store_match_ge;eauto;eapply program_equiv_symbol_address1;eauto).
-      rewrite <- H3. do 3 f_equal.
-      unfold eval_addrmode32.
-      destruct a. f_equal.
-      f_equal. destr.
-      destruct p0. eapply program_equiv_symbol_address1;eauto.
-      rewrite <- H3. do 3 f_equal.
-      unfold eval_addrmode64.
-      destruct a. f_equal.
-      f_equal. destr.
-      destruct p0. eapply program_equiv_symbol_address1;eauto.
+      destruct i;simpl in *;auto.      
+      1-24: try (erewrite program_equiv_symbol_address1;eauto).
+      1-21: try (erewrite exec_load_match_ge;eauto;eapply program_equiv_symbol_address1;eauto).
+      1-10: try (erewrite exec_store_match_ge;eauto;eapply program_equiv_symbol_address1;eauto).
 
-  (* - eapply exec_step_builtin with (vargs:= vargs);eauto. *)
-  (*   + unfold RelocProgGlobalenvs.Genv.find_ext_funct in *. *)
-  (*     destr. erewrite program_equiv_ext_funs1 in H1. *)
-  (*     eauto. eauto. *)
-  (*   + unfold RelocProgGlobalenvs.Genv.find_instr. *)
-  (*     erewrite program_equiv_instr_map. *)
-  (*     eauto. eapply program_equiv_sym. eauto. *)
-  (*   + eapply eval_builtin_args_match_ge. *)
-  (*     eapply program_equiv_symbol_address1;eauto. *)
-  (*     eauto. *)
-  (*   + eapply external_call_symbols_preserved with (ge1:= (Genv.genv_senv (RelocProgSemantics.globalenv instr_size p))). *)
-  (*     simpl. erewrite pe_prog_senv. *)
-  (*     unfold Senv.equiv. split;eauto. *)
-  (*     auto. auto. *)
+      erewrite high_half_match_ge;eauto;eapply program_equiv_symbol_address1;eauto.
       
   - eapply exec_step_external;eauto.
     + unfold RelocProgGlobalenvs.Genv.find_ext_funct in *.
@@ -175,14 +167,11 @@ Proof.
   intros.
   inv H0.
   set (ge' := RelocProgGlobalenvs.globalenv instr_size (decode_program instr_size tp)).
-  set (rs0' :=  ((rs # PC <-
+  set (rs0' :=(((Pregmap.init Vundef) # PC <-
            (Genv.symbol_address ge' (RelocProg.prog_main (decode_program instr_size tp)) Ptrofs.zero))
-          # RA <- Vnullptr) # RSP <-
-         (Vptr stk
-            (Ptrofs.sub (Ptrofs.repr (max_stacksize + align (size_chunk Mptr) 8))
-               (Ptrofs.repr (size_chunk Mptr))))).
+          # X2 <- Vnullptr) # X1 <- Vnullptr).
   
-  exists (State rs0' m2). split;auto.
+  exists (State rs0' m). split;auto.
   econstructor;eauto.
   f_equal.
   unfold rs0,rs0'.
