x86/RelocElfgenproofArchi.v
@@ -1,11 +1,11 @@
 Require Import Coqlib Maps AST lib.Integers Values.
 Require Import Events lib.Floats Memory Smallstep.
-Require Import Asm RelocProg RelocProgramBytes RelocElf Globalenvs.
+Require Import Asm RelocProg RelocProgramBytes RelocElf RelocElfArchi Globalenvs.
 Require Import Linking RelocProgLinking RelocElfLinking Errors.
 Require Import EncDecRet RelocElfgen LocalLib RelocProgGlobalenvs.
 Require Import RelocProgSemantics RelocProgSemantics1.
 Require Import RelocProgSemantics2 RelocElfSemantics.
-Require Import SymbtableDecode ReloctablesEncode.
+Require Import SymbtableDecode ReloctablesEncode ReloctablesDecode.
 Require Import RelocProgSemanticsArchi.
 Require Import ReloctablesEncodeArchi.
 Require Import RelocElfgenproof0.
@@ -18,6 +18,44 @@ Local Open Scope error_monad_scope.
 Local Open Scope hex_scope.
 Local Open Scope bits_scope.
 Local Open Scope string_byte_scope.
+
+
+Lemma decode_encode_reloctable_correct: forall n l bs m1 m2 (M: match_idxmap m1 m2),
+    (* let reloclen := if Archi.ptr64 then 24%nat else 8%nat in *)
+    length l = n ->
+    encode_reloctable m1 l = OK bs ->
+    fold_left (acc_decode_reloctable_section reloc_entry_size m2) bs (OK ([], [], 1%nat)) = OK (l, [], 1%nat).
+Proof.
+  induction n;intros.
+  rewrite length_zero_iff_nil in H. subst.
+  simpl in H0. inv H0.
+  unfold decode_reloctable_section. simpl. auto.
+
+  exploit LocalLib.length_S_inv;eauto.
+  intros (l' & a1 & A1 & B1). subst.
+  clear H.
+  unfold encode_reloctable in H0. rewrite fold_left_app in H0.
+  simpl in H0. unfold acc_reloctable in H0 at 1.
+  monadInv H0. exploit IHn;eauto.
+  intros. rewrite fold_left_app.
+
+  rewrite H. clear H EQ IHn.
+  exploit encode_relocentry_len;eauto.
+  eapply encode_reloc_info_len.  
+  intros LEN. 
+  rename x0 into l.
+  clear x.
+  eapply (ReloctablesDecodeArchi.decode_encode_relocentry encode_reloc_info decode_reloc_info) in EQ1;eauto.
+  2: eapply encode_reloc_info_len.
+  2: eapply decode_encode_reloc_info.
+
+  unfold acc_decode_reloctable_section. unfold reloc_entry_size.
+  destruct Archi.ptr64.
+  - do 25 (destruct l as [| ?b ?] ;simpl in LEN;try congruence).
+    simpl in *. rewrite EQ1. simpl. auto.
+  - do 9 (destruct l as [| ?b ?] ;simpl in LEN;try congruence).
+    simpl in *. rewrite EQ1. simpl. auto.
+Qed.
 
 
 Section WITH_INSTR_SIZE.
@@ -90,6 +128,7 @@ Proof.
   intros.
   unfold ge,tge in *.
   exploit gen_reloc_elf_correct;eauto.
+  eapply decode_encode_reloctable_correct.
   unfold globalenv.
   intros (p' & D1 & E1).
   rewrite D1.
